WIP

NuInstructions.thy
@@ -1,47 +1,62 @@
 theory NuInstructions
   imports NuSys NuBasicAbstractors
+  keywords
+    "myconsider" :: prf_goal % "proof"
 begin
 
-definition op_add :: "nat \<Rightarrow> ('a::len) word \<times> ('a::len) word \<times> 'r \<Rightarrow> (('a::len) word \<times> 'r) state"
+definition op_add :: "nat \<Rightarrow> ('a::len) word \<times> ('a::len) word \<times> ('r::lrep) \<Rightarrow> (('a::len) word \<times> 'r) state"
   where "op_add w p = (case p of (a,b,r) \<Rightarrow> if LENGTH('a) = w then StatOn (a+b, r) else STrap)"
 declare op_add_def[\<nu>instr]
 \<nu>overloads "+" and round_add and hehe
-theorem add_nat[\<nu>overload +]: "x + y < 2^LENGTH('b) \<Longrightarrow> \<^bold>p\<^bold>r\<^bold>o\<^bold>c op_add (LENGTH('b)) \<blangle> x \<tycolon> \<nat>['b::len] \<boxbar> y \<tycolon> \<nat>['b] \<boxbar> \<RR>emain_stack \<longmapsto> x + y \<tycolon> \<nat>['b] \<boxbar> \<RR>emain_stack \<brangle>"
+theorem add_nat[\<nu>overload +]: "\<^bold>p\<^bold>r\<^bold>e\<^bold>m\<^bold>i\<^bold>s\<^bold>e x + y < 2^LENGTH('b) \<Longrightarrow> \<^bold>p\<^bold>r\<^bold>o\<^bold>c op_add (LENGTH('b)) \<blangle> x \<tycolon> \<nat>['b::len] \<boxbar> y \<tycolon> \<nat>['b] \<boxbar> \<RR>emain_stack \<longmapsto> x + y \<tycolon> \<nat>['b] \<boxbar> \<RR>emain_stack \<brangle>"
   unfolding op_add_def Procedure_def by auto
 
 theorem add_nat_mod[\<nu>overload round_add]: "\<^bold>p\<^bold>r\<^bold>o\<^bold>c op_add (LENGTH('b)) \<blangle> x \<tycolon> \<nat>['b::len] \<boxbar> y \<tycolon> \<nat>['b] \<boxbar> \<RR> \<longmapsto> (x + y mod 2^(LENGTH('b))) \<tycolon> \<nat>['b] \<boxbar> \<RR> \<brangle>"
   unfolding op_add_def Procedure_def by auto (metis of_nat_unat ucast_id unat_of_nat)
 
-proc add2[\<nu>overload hehe]: "(x \<tycolon> \<nat>[32], y \<tycolon> \<nat>[32])" \<longmapsto> "(x + x + y \<tycolon> \<nat>[32])"
-  if "x < 100" and "y < 100"
-begin
+ML \<open>val _ =
+  Outer_Syntax.command \<^command_keyword>\<open>myconsider\<close> "state cases rule"
+    (Parse_Spec.obtains >> @{print} >> (Toplevel.proof' o Obtain.consider_cmd));\<close>
+
+proc add3 : "((x \<tycolon> \<nat>[32]) named x, y \<tycolon> \<nat>[32])" \<longmapsto> "(x + x + y \<tycolon> \<nat>[32])"
+  includes show_more
+  if A[in_using]:"x < 100" and [in_using]:"y < 100"
+\<nu>obtain z2 where c: "x < z2" by auto
+\<nu>obtain z3 where c2: "x < z3" by auto
   \<bullet> x x y + +
+ML_val \<open>Assumption.all_assms_of @{context}\<close>
+  finish
+
+
+proc add2 : "(( x \<tycolon> \<nat>[32]) named x, y \<tycolon> \<nat>[32])" \<longmapsto> "(x + x + y \<tycolon> \<nat>[32])"
+  if "x < 100" and "y < 100"
+  \<nu>have x[in_using]: "x < 100 \<and> y < 100" using that by auto
+  \<bullet> x x y +
+    \<nu>obtain z where c: "x < z" by auto
+  finish
+
+
+proc add2[\<nu>overload hehe]: "(( x \<tycolon> \<nat>[32]) named x, y \<tycolon> \<nat>[32])" \<longmapsto> "(x + x + y \<tycolon> \<nat>[32])"
+if A[in_using]:"x < 100" and [in_using]:"y < 100"
+    \<bullet> x x y + +
+    \<nu>obtain z where c: "x < z" by auto
 finish
 thm add2_\<nu>proc
-term "\<^bold>o\<^bold>b\<^bold>l\<^bold>i\<^bold>g\<^bold>a\<^bold>t\<^bold>i\<^bold>o\<^bold>n a"
 
-proc add3: "(x \<tycolon> \<nat>[32] named x, y \<tycolon> \<nat>[32])" \<longmapsto> "(x + x + y \<tycolon> \<nat>[32])" for x :: nat if A:"x < 100" and B:"y < 100" begin
-  \<bullet> y x hehe
-finish
 
-thm add3_\<nu>compilation
+proc add3: "(x \<tycolon> \<nat>[32], y \<tycolon> \<nat>[32])" \<longmapsto> "(x + x + y \<tycolon> \<nat>[32])"
+  if [in_using]:"x < 100" and [in_using]:"y < 100"
+  \<bullet> x x y + +
+  \<nu>have gg: "x < 200"  by auto
+  finish
+thm add3_\<nu>proc
 
-ML \<open>NuProcedure.check (Context.Proof @{context}) ("add2", Position.none)\<close>
-thm [[\<nu>overload add2]]
-ML \<open>NuProcedure.compilation_thm (Context.Proof @{context}) @{term add2}\<close>
+thm add3_\<nu>proc
 
-qed
-  show 
-  proof -
- qed
-  show ?thesis by this
-qed
-  then show ?thesis
-    by fast
-ML_val \<open>Thm.prop_of @{thm this}\<close>
-  ML_prf \<open>@{thm obli} RS @{thm this}\<close>
 
-qed
-  ML_val \<open>Proof_Context.read_term_schematic @{context} "?\<p>\<r>\<o>\<c>"\<close>
-  term ?\<p>\<r>\<o>\<c> 
 
+
+thm add2_\<nu>proc
+
+ML \<open>map (Attrib.attribute @{context}) @{attributes [elim]}\<close>
+end
