NuSys.thy
@@ -3,16 +3,21 @@
 theory NuSys
   imports NuPrim NuSyntax
   keywords
-    "proc" :: thy_decl_block
+    "proc" :: thy_goal_stmt
   and "\<medium_left_bracket>" "as" "\<rightarrow>" "\<longmapsto>" :: quasi_command
-  and "\<bullet>" "premise" :: prf_decl % "proof"
+  and "\<bullet>" "premise" "\<nu>have" "\<nu>obtain" :: prf_decl % "proof"
   and "\<nu>processor" "\<nu>processor_resolver" :: thy_decl % "ML"
   and "\<nu>overloads" :: thy_decl
-and "finish" :: qed_block % "proof"
+  and "finish" :: "qed" % "proof"
 (*   and "finish" :: qed_block % "proof" *)
 abbrevs
   "!!" = "!!"
 begin
+
+named_theorems in_using \<open>theorems that will be inserted in ANY proof environments.\<close>
+  and final_proc_rewrite \<open>rules used to rewrite the generated procedure theorem in the final stage\<close>
+declare Premise_Irew[final_proc_rewrite]
+
 
 ML_file_debug NuHelp.ML
 ML_file "./general/binary_tree.ML"
@@ -28,7 +33,7 @@ ML_file "./library/processors.ML"
 ML_file "./library/procedure.ML"
 ML_file NuSys.ML
 ML_file_debug NuToplevel.ML
-
+ML_file "./library/obtain.ML"
 
 ML \<open>Theory.setup (Global_Theory.add_thms_dynamic (@{binding "\<nu>instr"}, NuInstructions.list_definitions #> map snd))  \<close>
 attribute_setup \<nu>instr = \<open>Scan.succeed (Thm.declaration_attribute NuInstructions.add) \<close>
@@ -40,13 +45,18 @@ attribute_setup show_proc_expression = \<open>NuToplevel.show_proc_expression_at
 
 ML \<open>
 
-local open Scan NuToplevel NuSys Parse in
+local open Scan NuToplevel NuSys Parse 
+val nustatement = Parse.and_list1 (Parse_Spec.thm_name ":" -- opt_attribs -- Scan.repeat1 Parse.propp);
+val structured_statement =
+  nustatement -- Parse_Spec.if_statement' -- Parse.for_fixes
+    >> (fn ((shows, assumes), fixes) => (fixes, assumes, shows));
 val bracket_begin = $$$ "\<medium_left_bracket>";
+in
 
 val _ =
   Outer_Syntax.local_theory_to_proof' \<^command_keyword>\<open>proc\<close> "begin a procedure construction"
     ((Parse_Spec.thm_name ":" -- Parse.term --| $$$ "\<longmapsto>" -- Parse.term -- Parse.for_fixes -- Scan.optional Parse_Spec.includes []
-            -- Parse_Spec.if_statement) --| $$$ "begin" >>
+            -- Parse_Spec.if_statement) >>
         (fn (((((b,arg),ret),fixes),includes),preconds) =>  
             (begin_proc_cmd b arg ret fixes includes preconds)));
 
@@ -60,7 +70,17 @@ val _ =
 
 val _ =
   Outer_Syntax.command \<^command_keyword>\<open>premise\<close> "proof for premise"
-    (Scan.succeed (Toplevel.proof NuToplevel.prove_prem))
+    (Scan.succeed (Toplevel.proof' (snd oo NuToplevel.prove_prem)))
+
+val _ =
+  Outer_Syntax.command \<^command_keyword>\<open>\<nu>have\<close> "proof for premise"
+    (and_list1 ((binding -- opt_attribs -- opt_attribs --| $$$ ":") -- and_list1 (prop -- repeat prop)) >>
+      (Toplevel.proof' o (snd ooo NuToplevel.have_aux_cmd)))
+
+val _ =
+  Outer_Syntax.command \<^command_keyword>\<open>\<nu>obtain\<close> "generalized elimination"
+    (Parse.parbinding -- Scan.optional (Parse.vars --| Parse.where_) [] -- structured_statement
+      >> (fn ((a, b), (c, d, e)) => Toplevel.proof' (NuObtain.obtain_cmd a b c d e)));
 
 val _ =
   Outer_Syntax.local_theory \<^command_keyword>\<open>\<nu>processor\<close> "define \<nu>processor"
@@ -84,8 +104,8 @@ end
 attribute_setup \<nu>overload = \<open>Scan.lift (Parse.and_list1 NuProcedure.parser) >> (fn bindings => 
   Thm.declaration_attribute (fn th => fold (NuProcedure.overload th) bindings))\<close>
 
-(* \<nu>processor set_auto_level 10 \<open>PROP P\<close> \<open>(fn auto_level => fn ctx => fn th => NuParse.auto_level_force #->
-  (fn auto_level' => NuProcessor.process (Int.min (auto_level, auto_level')) ctx th #> (fn x => raise ProcessTerminated x)))\<close> *)
+\<nu>processor set_auto_level 10 \<open>PROP P\<close> \<open>(fn ctx => fn th => NuParse.auto_level_force #->
+  (fn auto_level' => NuProcessor.process (AutoLevel.reduce auto_level' ctx) th #> (fn x => raise ProcessTerminated x)))\<close>
 \<nu>processor accept_proc 300 \<open>\<^bold>p\<^bold>e\<^bold>n\<^bold>d\<^bold>i\<^bold>n\<^bold>g f \<^bold>o\<^bold>n blk \<^bold>r\<^bold>e\<^bold>s\<^bold>u\<^bold>l\<^bold>t\<^bold>s \<^bold>i\<^bold>n T\<close> \<open>Scan.succeed oo NuSys.accept_proc\<close>
 \<nu>processor assign_register 500 \<open>\<^bold>c\<^bold>u\<^bold>r\<^bold>r\<^bold>e\<^bold>n\<^bold>t blk \<^bold>r\<^bold>e\<^bold>s\<^bold>u\<^bold>l\<^bold>t\<^bold>s \<^bold>i\<^bold>n T\<close>  \<open>let open Parse in
   (fn ctx => fn th => ($$$ "\<rightarrow>" |-- (short_ident >> single || $$$ "(" |-- list1 short_ident --| $$$ ")")) >>
@@ -96,13 +116,11 @@ end\<close>
       handle NuRegisters.NoSuchRegister _ => raise Bypass)
 end\<close>
 \<nu>processor \<nu>simplifier 40 \<open>\<^bold>c\<^bold>u\<^bold>r\<^bold>r\<^bold>e\<^bold>n\<^bold>t blk \<^bold>r\<^bold>e\<^bold>s\<^bold>u\<^bold>l\<^bold>t\<^bold>s \<^bold>i\<^bold>n T\<close>  \<open>NuProcessors.simplifier\<close>
-\<nu>processor \<nu>autoprover 9000 \<open>P \<Longrightarrow> PROP Q\<close>
-  \<open>let open Tactical Method in 
-    premise_prover (not_safe (fn ctx => SOLVED' (K (ALLGOALS (insert_tac ctx (Proof_Context.get_thms ctx "that")) THEN Simpdata.auto_tac ctx)) 0))
-  end\<close>
+\<nu>processor \<nu>autoprover 9000 \<open>\<^bold>p\<^bold>r\<^bold>e\<^bold>m\<^bold>i\<^bold>s\<^bold>e P \<Longrightarrow> PROP Q\<close> \<open>premise_prover (not_safe NuSys.premise_tac)\<close>
 \<nu>processor call 9000 \<open>\<^bold>c\<^bold>u\<^bold>r\<^bold>r\<^bold>e\<^bold>n\<^bold>t blk \<^bold>r\<^bold>e\<^bold>s\<^bold>u\<^bold>l\<^bold>t\<^bold>s \<^bold>i\<^bold>n T\<close> \<open> fn ctx => fn focus => NuProcedure.parser >> (fn binding =>
     NuSys.apply_procs ctx (NuProcedure.procedure_thm ctx binding) focus)\<close>
 
 \<nu>processor_resolver resolve_disposable 100  \<open>\<nu>Disposable T \<Longrightarrow> PROP P\<close> \<nu>disposable
 \<nu>processor_resolver resolve_share 100  \<open>Nu_Share N sh f \<Longrightarrow> PROP P\<close> \<nu>share
+ML \<open>Goal.init @{cterm "A \<Longrightarrow> B"}\<close>
 end
